<?xml version="1.0"?>
<rdf:RDF xmlns="http://purl.obolibrary.org/obo/foodon/imports/ro_import.owl#"
     xml:base="http://purl.obolibrary.org/obo/foodon/imports/ro_import.owl"
     xmlns:obo="http://purl.obolibrary.org/obo/"
     xmlns:owl="http://www.w3.org/2002/07/owl#"
     xmlns:rdf="http://www.w3.org/1999/02/22-rdf-syntax-ns#"
     xmlns:xml="http://www.w3.org/XML/1998/namespace"
     xmlns:xsd="http://www.w3.org/2001/XMLSchema#"
     xmlns:rdfs="http://www.w3.org/2000/01/rdf-schema#">
    <owl:Ontology rdf:about="http://purl.obolibrary.org/obo/foodon/imports/ro_import.owl"/>
    


    <!-- 
    ///////////////////////////////////////////////////////////////////////////////////////
    //
    // Annotation properties
    //
    ///////////////////////////////////////////////////////////////////////////////////////
     -->

    


    <!-- http://purl.obolibrary.org/obo/IAO_0000111 -->

    <!-- <owl:AnnotationProperty rdf:about="http://purl.obolibrary.org/obo/IAO_0000111">
        <rdfs:label xml:lang="en">editor preferred term</rdfs:label>
    </owl:AnnotationProperty> -->
    


    <!-- http://purl.obolibrary.org/obo/IAO_0000114 -->

    <!-- <owl:AnnotationProperty rdf:about="http://purl.obolibrary.org/obo/IAO_0000114">
        <rdfs:label xml:lang="en">has curation status</rdfs:label>
    </owl:AnnotationProperty> -->
    


    <!-- http://purl.obolibrary.org/obo/IAO_0000115 -->

    <!-- <owl:AnnotationProperty rdf:about="http://purl.obolibrary.org/obo/IAO_0000115">
        <obo:IAO_0000114 rdf:resource="http://purl.obolibrary.org/obo/IAO_0000122"/>
        <rdfs:label rdf:datatype="http://www.w3.org/2001/XMLSchema#string">definition</rdfs:label>
    </owl:AnnotationProperty> -->
    


    <!-- http://purl.obolibrary.org/obo/IAO_0000119 -->

    <!-- <owl:AnnotationProperty rdf:about="http://purl.obolibrary.org/obo/IAO_0000119">
        <obo:IAO_0000114 rdf:resource="http://purl.obolibrary.org/obo/IAO_0000122"/>
        <rdfs:label xml:lang="en">definition source</rdfs:label>
    </owl:AnnotationProperty> -->
    


    <!-- http://purl.obolibrary.org/obo/IAO_0000412 -->

    <!-- <owl:AnnotationProperty rdf:about="http://purl.obolibrary.org/obo/IAO_0000412">
        <rdfs:label xml:lang="en">imported from</rdfs:label>
    </owl:AnnotationProperty> -->
    


    <!-- http://www.w3.org/2000/01/rdf-schema#label -->

    <!-- <owl:AnnotationProperty rdf:about="http://www.w3.org/2000/01/rdf-schema#label"/> -->
    


    <!-- 
    ///////////////////////////////////////////////////////////////////////////////////////
    //
    // Object Properties
    //
    ///////////////////////////////////////////////////////////////////////////////////////
     -->

    


    <!-- http://purl.obolibrary.org/obo/BFO_0000050 -->

    <owl:ObjectProperty rdf:about="http://purl.obolibrary.org/obo/BFO_0000050">
        <rdfs:subPropertyOf rdf:resource="http://purl.obolibrary.org/obo/RO_0002131"/>
        <rdf:type rdf:resource="http://www.w3.org/2002/07/owl#TransitiveProperty"/>
        <obo:IAO_0000111 xml:lang="en">is part of</obo:IAO_0000111>
        <obo:IAO_0000115 xml:lang="en">a core relation that holds between a part and its whole</obo:IAO_0000115>
        <obo:IAO_0000412 rdf:resource="http://purl.obolibrary.org/obo/ro.owl"/>
        <rdfs:label xml:lang="en">part of</rdfs:label>
    </owl:ObjectProperty>
    


    <!-- http://purl.obolibrary.org/obo/BFO_0000051 -->

    <owl:ObjectProperty rdf:about="http://purl.obolibrary.org/obo/BFO_0000051">
        <rdfs:subPropertyOf rdf:resource="http://purl.obolibrary.org/obo/RO_0002131"/>
        <rdf:type rdf:resource="http://www.w3.org/2002/07/owl#TransitiveProperty"/>
        <obo:IAO_0000111 xml:lang="en">has part</obo:IAO_0000111>
        <obo:IAO_0000115 xml:lang="en">a core relation that holds between a whole and its part</obo:IAO_0000115>
        <obo:IAO_0000412 rdf:resource="http://purl.obolibrary.org/obo/ro.owl"/>
        <rdfs:label xml:lang="en">has part</rdfs:label>
    </owl:ObjectProperty>
    


    <!-- http://purl.obolibrary.org/obo/BFO_0000054 -->

    <owl:ObjectProperty rdf:about="http://purl.obolibrary.org/obo/BFO_0000054">
        <obo:IAO_0000111 xml:lang="en">realized in</obo:IAO_0000111>
        <obo:IAO_0000412 rdf:resource="http://purl.obolibrary.org/obo/ro.owl"/>
        <rdfs:label xml:lang="en">realized in</rdfs:label>
    </owl:ObjectProperty>
    


    <!-- http://purl.obolibrary.org/obo/BFO_0000055 -->

    <owl:ObjectProperty rdf:about="http://purl.obolibrary.org/obo/BFO_0000055">
        <obo:IAO_0000111 xml:lang="en">realizes</obo:IAO_0000111>
        <obo:IAO_0000412 rdf:resource="http://purl.obolibrary.org/obo/ro.owl"/>
        <rdfs:label xml:lang="en">realizes</rdfs:label>
    </owl:ObjectProperty>
    


    <!-- http://purl.obolibrary.org/obo/RO_0000052 -->

    <owl:ObjectProperty rdf:about="http://purl.obolibrary.org/obo/RO_0000052">
        <rdfs:subPropertyOf rdf:resource="http://purl.obolibrary.org/obo/RO_0002314"/>
        <obo:IAO_0000111 xml:lang="en">inheres in</obo:IAO_0000111>
        <obo:IAO_0000115 xml:lang="en">a relation between a specifically dependent continuant (the dependent) and an independent continuant (the bearer), in which the dependent specifically depends on the bearer for its existence</obo:IAO_0000115>
        <obo:IAO_0000412 rdf:resource="http://purl.obolibrary.org/obo/ro.owl"/>
        <rdfs:label xml:lang="en">inheres in</rdfs:label>
    </owl:ObjectProperty>
    


    <!-- http://purl.obolibrary.org/obo/RO_0000053 -->

    <owl:ObjectProperty rdf:about="http://purl.obolibrary.org/obo/RO_0000053">
        <obo:IAO_0000111 xml:lang="en">bearer of</obo:IAO_0000111>
        <obo:IAO_0000115 xml:lang="en">a relation between an independent continuant (the bearer) and a specifically dependent continuant (the dependent), in which the dependent specifically depends on the bearer for its existence</obo:IAO_0000115>
        <obo:IAO_0000412 rdf:resource="http://purl.obolibrary.org/obo/ro.owl"/>
        <rdfs:label xml:lang="en">bearer of</rdfs:label>
    </owl:ObjectProperty>
    


    <!-- http://purl.obolibrary.org/obo/RO_0000056 -->

    <owl:ObjectProperty rdf:about="http://purl.obolibrary.org/obo/RO_0000056">
        <obo:IAO_0000111 xml:lang="en">participates in</obo:IAO_0000111>
        <obo:IAO_0000115 xml:lang="en">a relation between a continuant and a process, in which the continuant is somehow involved in the process</obo:IAO_0000115>
        <obo:IAO_0000412 rdf:resource="http://purl.obolibrary.org/obo/ro.owl"/>
        <rdfs:label xml:lang="en">participates in</rdfs:label>
    </owl:ObjectProperty>
    


    <!-- http://purl.obolibrary.org/obo/RO_0000057 -->

    <owl:ObjectProperty rdf:about="http://purl.obolibrary.org/obo/RO_0000057">
        <obo:IAO_0000111 xml:lang="en">has participant</obo:IAO_0000111>
        <obo:IAO_0000115 xml:lang="en">a relation between a process and a continuant, in which the continuant is somehow involved in the process</obo:IAO_0000115>
        <obo:IAO_0000412 rdf:resource="http://purl.obolibrary.org/obo/ro.owl"/>
        <rdfs:label xml:lang="en">has participant</rdfs:label>
    </owl:ObjectProperty>
    


    <!-- http://purl.obolibrary.org/obo/RO_0000079 -->

    <owl:ObjectProperty rdf:about="http://purl.obolibrary.org/obo/RO_0000079">
        <rdfs:subPropertyOf rdf:resource="http://purl.obolibrary.org/obo/RO_0000052"/>
        <obo:IAO_0000115 xml:lang="en">a relation between a function and an independent continuant (the bearer), in which the function specifically depends on the bearer for its existence</obo:IAO_0000115>
        <obo:IAO_0000412 rdf:resource="http://purl.obolibrary.org/obo/ro.owl"/>
        <rdfs:label xml:lang="en">function of</rdfs:label>
    </owl:ObjectProperty>
    


    <!-- http://purl.obolibrary.org/obo/RO_0000080 -->

    <owl:ObjectProperty rdf:about="http://purl.obolibrary.org/obo/RO_0000080">
        <rdfs:subPropertyOf rdf:resource="http://purl.obolibrary.org/obo/RO_0000052"/>
        <obo:IAO_0000115 xml:lang="en">a relation between a quality and an independent continuant (the bearer), in which the quality specifically depends on the bearer for its existence</obo:IAO_0000115>
        <obo:IAO_0000412 rdf:resource="http://purl.obolibrary.org/obo/ro.owl"/>
        <rdfs:label xml:lang="en">quality of</rdfs:label>
    </owl:ObjectProperty>
    


    <!-- http://purl.obolibrary.org/obo/RO_0000081 -->

    <owl:ObjectProperty rdf:about="http://purl.obolibrary.org/obo/RO_0000081">
        <rdfs:subPropertyOf rdf:resource="http://purl.obolibrary.org/obo/RO_0000052"/>
        <obo:IAO_0000115 xml:lang="en">a relation between a role and an independent continuant (the bearer), in which the role specifically depends on the bearer for its existence</obo:IAO_0000115>
        <obo:IAO_0000412 rdf:resource="http://purl.obolibrary.org/obo/ro.owl"/>
        <rdfs:label xml:lang="en">role of</rdfs:label>
    </owl:ObjectProperty>
    


    <!-- http://purl.obolibrary.org/obo/RO_0000085 -->

    <owl:ObjectProperty rdf:about="http://purl.obolibrary.org/obo/RO_0000085">
        <rdfs:subPropertyOf rdf:resource="http://purl.obolibrary.org/obo/RO_0000053"/>
        <obo:IAO_0000115 xml:lang="en">a relation between an independent continuant (the bearer) and a function, in which the function specifically depends on the bearer for its existence</obo:IAO_0000115>
        <obo:IAO_0000412 rdf:resource="http://purl.obolibrary.org/obo/ro.owl"/>
        <rdfs:label xml:lang="en">has function</rdfs:label>
    </owl:ObjectProperty>
    


    <!-- http://purl.obolibrary.org/obo/RO_0000086 -->

    <owl:ObjectProperty rdf:about="http://purl.obolibrary.org/obo/RO_0000086">
        <rdfs:subPropertyOf rdf:resource="http://purl.obolibrary.org/obo/RO_0000053"/>
        <obo:IAO_0000115 xml:lang="en">a relation between an independent continuant (the bearer) and a quality, in which the quality specifically depends on the bearer for its existence</obo:IAO_0000115>
        <obo:IAO_0000412 rdf:resource="http://purl.obolibrary.org/obo/ro.owl"/>
        <rdfs:label xml:lang="en">has quality</rdfs:label>
    </owl:ObjectProperty>
    


    <!-- http://purl.obolibrary.org/obo/RO_0000087 -->

    <owl:ObjectProperty rdf:about="http://purl.obolibrary.org/obo/RO_0000087">
        <rdfs:subPropertyOf rdf:resource="http://purl.obolibrary.org/obo/RO_0000053"/>
        <obo:IAO_0000115 xml:lang="en">a relation between an independent continuant (the bearer) and a role, in which the role specifically depends on the bearer for its existence</obo:IAO_0000115>
        <obo:IAO_0000412 rdf:resource="http://purl.obolibrary.org/obo/ro.owl"/>
        <rdfs:label xml:lang="en">has role</rdfs:label>
    </owl:ObjectProperty>
    


    <!-- http://purl.obolibrary.org/obo/RO_0000092 -->

    <owl:ObjectProperty rdf:about="http://purl.obolibrary.org/obo/RO_0000092">
        <rdfs:subPropertyOf rdf:resource="http://purl.obolibrary.org/obo/RO_0000052"/>
        <obo:IAO_0000115>inverse of has disposition</obo:IAO_0000115>
        <obo:IAO_0000412 rdf:resource="http://purl.obolibrary.org/obo/ro.owl"/>
        <rdfs:label xml:lang="en">disposition of</rdfs:label>
    </owl:ObjectProperty>
    


    <!-- http://purl.obolibrary.org/obo/RO_0001000 -->

    <owl:ObjectProperty rdf:about="http://purl.obolibrary.org/obo/RO_0001000">
        <obo:IAO_0000114 rdf:resource="http://purl.obolibrary.org/obo/IAO_0000125"/>
        <obo:IAO_0000115 xml:lang="en">a relation between two distinct material entities, the new entity and the old entity, in which the new entity begins to exist when the old entity ceases to exist, and the new entity inherits the significant portion of the matter of the old entity</obo:IAO_0000115>
        <obo:IAO_0000412 rdf:resource="http://purl.obolibrary.org/obo/ro.owl"/>
        <rdfs:label xml:lang="en">derives from</rdfs:label>
    </owl:ObjectProperty>
    


    <!-- http://purl.obolibrary.org/obo/RO_0001001 -->

    <owl:ObjectProperty rdf:about="http://purl.obolibrary.org/obo/RO_0001001">
        <obo:IAO_0000114 rdf:resource="http://purl.obolibrary.org/obo/IAO_0000125"/>
        <obo:IAO_0000115 xml:lang="en">a relation between two distinct material entities, the old entity and the new entity, in which the new entity begins to exist when the old entity ceases to exist, and the new entity inherits the significant portion of the matter of the old entity</obo:IAO_0000115>
        <obo:IAO_0000412 rdf:resource="http://purl.obolibrary.org/obo/ro.owl"/>
        <rdfs:label xml:lang="en">derives into</rdfs:label>
    </owl:ObjectProperty>
    


    <!-- http://purl.obolibrary.org/obo/RO_0001020 -->

    <owl:ObjectProperty rdf:about="http://purl.obolibrary.org/obo/RO_0001020">
        <rdfs:subPropertyOf rdf:resource="http://purl.obolibrary.org/obo/RO_0003302"/>
        <obo:IAO_0000115>A relation between a material entity and a condition (a phenotype or disease) of a host, in which the material entity is not part of the host, and is considered harmless to non-allergic hosts, and the condition results in pathological processes that include an abnormally strong immune response against the material entity.</obo:IAO_0000115>
        <obo:IAO_0000412 rdf:resource="http://purl.obolibrary.org/obo/ro.owl"/>
        <rdfs:label xml:lang="en">is allergic trigger for</rdfs:label>
    </owl:ObjectProperty>
    


    <!-- http://purl.obolibrary.org/obo/RO_0001022 -->

    <owl:ObjectProperty rdf:about="http://purl.obolibrary.org/obo/RO_0001022">
        <rdfs:subPropertyOf rdf:resource="http://purl.obolibrary.org/obo/RO_0003302"/>
        <obo:IAO_0000115>A relation between a condition (a phenotype or disease) of a host and a material entity, in which the material entity is not part of the host, and is considered harmless to non-allergic hosts, and the condition results in pathological processes that include an abnormally strong immune response against the material entity.</obo:IAO_0000115>
        <obo:IAO_0000412 rdf:resource="http://purl.obolibrary.org/obo/ro.owl"/>
        <rdfs:label xml:lang="en">has allergic trigger</rdfs:label>
    </owl:ObjectProperty>
    


    <!-- http://purl.obolibrary.org/obo/RO_0001025 -->

    <owl:ObjectProperty rdf:about="http://purl.obolibrary.org/obo/RO_0001025">
        <rdf:type rdf:resource="http://www.w3.org/2002/07/owl#TransitiveProperty"/>
        <obo:IAO_0000111 xml:lang="en">located in</obo:IAO_0000111>
        <obo:IAO_0000115 xml:lang="en">a relation between two independent continuants, the target and the location, in which the target is entirely within the location</obo:IAO_0000115>
        <obo:IAO_0000412 rdf:resource="http://purl.obolibrary.org/obo/ro.owl"/>
        <rdfs:label xml:lang="en">located in</rdfs:label>
    </owl:ObjectProperty>
    


    <!-- http://purl.obolibrary.org/obo/RO_0002131 -->

    <owl:ObjectProperty rdf:about="http://purl.obolibrary.org/obo/RO_0002131">
        <rdfs:subPropertyOf rdf:resource="http://purl.obolibrary.org/obo/RO_0002323"/>
        <obo:IAO_0000114 rdf:resource="http://purl.obolibrary.org/obo/IAO_0000125"/>
        <obo:IAO_0000115>x overlaps y if and only if there exists some z such that x has part z and z part of y</obo:IAO_0000115>
        <obo:IAO_0000412 rdf:resource="http://purl.obolibrary.org/obo/ro.owl"/>
        <rdfs:label xml:lang="en">overlaps</rdfs:label>
    </owl:ObjectProperty>
    


    <!-- http://purl.obolibrary.org/obo/RO_0002162 -->

    <owl:ObjectProperty rdf:about="http://purl.obolibrary.org/obo/RO_0002162">
        <rdfs:subPropertyOf rdf:resource="http://purl.obolibrary.org/obo/RO_0002320"/>
        <obo:IAO_0000114 rdf:resource="http://purl.obolibrary.org/obo/IAO_0000125"/>
        <obo:IAO_0000115>x is in taxon y if an only if y is an organism, and the relationship between x and y is one of: part of (reflexive), developmentally preceded by, derives from, secreted by, expressed.</obo:IAO_0000115>
        <obo:IAO_0000119 rdf:resource="http://www.ncbi.nlm.nih.gov/pubmed/17921072"/>
        <obo:IAO_0000119 rdf:resource="http://www.ncbi.nlm.nih.gov/pubmed/20973947"/>
        <obo:IAO_0000412 rdf:resource="http://purl.obolibrary.org/obo/ro.owl"/>
        <rdfs:label rdf:datatype="http://www.w3.org/2001/XMLSchema#string">in taxon</rdfs:label>
    </owl:ObjectProperty>
    


    <!-- http://purl.obolibrary.org/obo/RO_0002163 -->

    <owl:ObjectProperty rdf:about="http://purl.obolibrary.org/obo/RO_0002163">
        <rdfs:subPropertyOf rdf:resource="http://purl.obolibrary.org/obo/RO_0002323"/>
        <obo:IAO_0000114 rdf:resource="http://purl.obolibrary.org/obo/IAO_0000125"/>
        <obo:IAO_0000115>A is spatially_disjoint_from B if and only if they have no parts in common</obo:IAO_0000115>
        <obo:IAO_0000119 rdf:resource="http://www.ncbi.nlm.nih.gov/pubmed/22293552"/>
        <obo:IAO_0000412 rdf:resource="http://purl.obolibrary.org/obo/ro.owl"/>
        <rdfs:label rdf:datatype="http://www.w3.org/2001/XMLSchema#string">spatially disjoint from</rdfs:label>
    </owl:ObjectProperty>
    


    <!-- http://purl.obolibrary.org/obo/RO_0002215 -->

    <owl:ObjectProperty rdf:about="http://purl.obolibrary.org/obo/RO_0002215">
        <rdfs:subPropertyOf rdf:resource="http://purl.obolibrary.org/obo/RO_0002216"/>
        <obo:IAO_0000115>A relation between a material entity (such as a cell) and a process, in which the material entity has the ability to carry out the process. </obo:IAO_0000115>
        <obo:IAO_0000119 rdf:resource="http://www.ncbi.nlm.nih.gov/pubmed/20123131"/>
        <obo:IAO_0000119 rdf:resource="http://www.ncbi.nlm.nih.gov/pubmed/21208450"/>
        <obo:IAO_0000412 rdf:resource="http://purl.obolibrary.org/obo/ro.owl"/>
        <rdfs:label xml:lang="en">capable of</rdfs:label>
    </owl:ObjectProperty>
    


    <!-- http://purl.obolibrary.org/obo/RO_0002216 -->

    <owl:ObjectProperty rdf:about="http://purl.obolibrary.org/obo/RO_0002216">
        <rdfs:subPropertyOf rdf:resource="http://purl.obolibrary.org/obo/RO_0002328"/>
        <rdfs:subPropertyOf rdf:resource="http://purl.obolibrary.org/obo/RO_0002500"/>
        <obo:IAO_0000115>c stands in this relationship to p if and only if there exists some p&apos; such that c is capable_of p&apos;, and p&apos; is part_of p.</obo:IAO_0000115>
        <obo:IAO_0000412 rdf:resource="http://purl.obolibrary.org/obo/ro.owl"/>
        <rdfs:label xml:lang="en">capable of part of</rdfs:label>
    </owl:ObjectProperty>
    


    <!-- http://purl.obolibrary.org/obo/RO_0002219 -->

    <owl:ObjectProperty rdf:about="http://purl.obolibrary.org/obo/RO_0002219">
        <rdfs:subPropertyOf rdf:resource="http://purl.obolibrary.org/obo/RO_0002220"/>
        <obo:IAO_0000114 rdf:resource="http://purl.obolibrary.org/obo/IAO_0000125"/>
        <obo:IAO_0000115>x surrounded_by y if and only if (1) x is adjacent to y and for every region r that is adjacent to x, r overlaps y (2) the shared boundary between x and y occupies the majority of the outermost boundary of x</obo:IAO_0000115>
        <obo:IAO_0000412 rdf:resource="http://purl.obolibrary.org/obo/ro.owl"/>
        <rdfs:label xml:lang="en">surrounded by</rdfs:label>
    </owl:ObjectProperty>
    


    <!-- http://purl.obolibrary.org/obo/RO_0002220 -->

    <owl:ObjectProperty rdf:about="http://purl.obolibrary.org/obo/RO_0002220">
        <rdfs:subPropertyOf rdf:resource="http://purl.obolibrary.org/obo/RO_0002163"/>
        <obo:IAO_0000114 rdf:resource="http://purl.obolibrary.org/obo/IAO_0000125"/>
        <obo:IAO_0000115>x adjacent to y if and only if x and y share a boundary.</obo:IAO_0000115>
        <obo:IAO_0000412 rdf:resource="http://purl.obolibrary.org/obo/ro.owl"/>
        <rdfs:label xml:lang="en">adjacent to</rdfs:label>
    </owl:ObjectProperty>
    


    <!-- http://purl.obolibrary.org/obo/RO_0002221 -->

    <owl:ObjectProperty rdf:about="http://purl.obolibrary.org/obo/RO_0002221">
        <rdfs:subPropertyOf rdf:resource="http://purl.obolibrary.org/obo/RO_0002220"/>
        <obo:IAO_0000114 rdf:resource="http://purl.obolibrary.org/obo/IAO_0000125"/>
        <obo:IAO_0000115>inverse of surrounded by</obo:IAO_0000115>
        <obo:IAO_0000412 rdf:resource="http://purl.obolibrary.org/obo/ro.owl"/>
        <rdfs:label xml:lang="en">surrounds</rdfs:label>
    </owl:ObjectProperty>
    


    <!-- http://purl.obolibrary.org/obo/RO_0002222 -->

    <owl:ObjectProperty rdf:about="http://purl.obolibrary.org/obo/RO_0002222">
        <obo:IAO_0000114 rdf:resource="http://purl.obolibrary.org/obo/IAO_0000125"/>
        <obo:IAO_0000119 rdf:resource="https://en.wikipedia.org/wiki/Allen%27s_interval_algebra"/>
        <obo:IAO_0000412 rdf:resource="http://purl.obolibrary.org/obo/ro.owl"/>
        <rdfs:label xml:lang="en">temporally related to</rdfs:label>
    </owl:ObjectProperty>
    


    <!-- http://purl.obolibrary.org/obo/RO_0002224 -->

    <owl:ObjectProperty rdf:about="http://purl.obolibrary.org/obo/RO_0002224">
        <rdfs:subPropertyOf rdf:resource="http://purl.obolibrary.org/obo/BFO_0000051"/>
        <rdfs:subPropertyOf rdf:resource="http://purl.obolibrary.org/obo/RO_0002222"/>
        <rdf:type rdf:resource="http://www.w3.org/2002/07/owl#TransitiveProperty"/>
        <obo:IAO_0000114 rdf:resource="http://purl.obolibrary.org/obo/IAO_0000125"/>
        <obo:IAO_0000115>x starts with y if and only if x has part y and the time point at which x starts is equivalent to the time point at which y starts. Formally: α(y) = α(x) ∧ ω(y) &lt; ω(x), where α is a function that maps a process to a start point, and ω is a function that maps a process to an end point.</obo:IAO_0000115>
        <obo:IAO_0000412 rdf:resource="http://purl.obolibrary.org/obo/ro.owl"/>
        <rdfs:label xml:lang="en">starts with</rdfs:label>
    </owl:ObjectProperty>
    


    <!-- http://purl.obolibrary.org/obo/RO_0002230 -->

    <owl:ObjectProperty rdf:about="http://purl.obolibrary.org/obo/RO_0002230">
        <rdfs:subPropertyOf rdf:resource="http://purl.obolibrary.org/obo/BFO_0000051"/>
        <rdfs:subPropertyOf rdf:resource="http://purl.obolibrary.org/obo/RO_0002222"/>
        <rdf:type rdf:resource="http://www.w3.org/2002/07/owl#TransitiveProperty"/>
        <obo:IAO_0000114 rdf:resource="http://purl.obolibrary.org/obo/IAO_0000125"/>
        <obo:IAO_0000115>x ends with y if and only if x has part y and the time point at which x ends is equivalent to the time point at which y ends. Formally: α(y) &gt; α(x) ∧ ω(y) = ω(x), where α is a function that maps a process to a start point, and ω is a function that maps a process to an end point.</obo:IAO_0000115>
        <obo:IAO_0000412 rdf:resource="http://purl.obolibrary.org/obo/ro.owl"/>
        <rdfs:label xml:lang="en">ends with</rdfs:label>
    </owl:ObjectProperty>
    


    <!-- http://purl.obolibrary.org/obo/RO_0002233 -->

    <owl:ObjectProperty rdf:about="http://purl.obolibrary.org/obo/RO_0002233">
        <rdfs:subPropertyOf rdf:resource="http://purl.obolibrary.org/obo/RO_0000057"/>
        <obo:IAO_0000114 rdf:resource="http://purl.obolibrary.org/obo/IAO_0000125"/>
        <obo:IAO_0000115>p has input c iff: p is a process, c is a material entity, c is a participant in p, c is present at the start of p, and the state of c is modified during p.</obo:IAO_0000115>
        <obo:IAO_0000412 rdf:resource="http://purl.obolibrary.org/obo/ro.owl"/>
        <rdfs:label xml:lang="en">has input</rdfs:label>
    </owl:ObjectProperty>
    


    <!-- http://purl.obolibrary.org/obo/RO_0002234 -->

    <owl:ObjectProperty rdf:about="http://purl.obolibrary.org/obo/RO_0002234">
        <rdfs:subPropertyOf rdf:resource="http://purl.obolibrary.org/obo/RO_0000057"/>
        <obo:IAO_0000114 rdf:resource="http://purl.obolibrary.org/obo/IAO_0000125"/>
        <obo:IAO_0000115>p has output c iff c is a participant in p, c is present at the end of p, and c is not present at the beginning of p.</obo:IAO_0000115>
        <obo:IAO_0000412 rdf:resource="http://purl.obolibrary.org/obo/ro.owl"/>
        <rdfs:label xml:lang="en">has output</rdfs:label>
    </owl:ObjectProperty>
    


    <!-- http://purl.obolibrary.org/obo/RO_0002314 -->

    <owl:ObjectProperty rdf:about="http://purl.obolibrary.org/obo/RO_0002314">
        <rdfs:subPropertyOf rdf:resource="http://purl.obolibrary.org/obo/RO_0002502"/>
        <obo:IAO_0000115>q inheres in part of w if and only if there exists some p such that q inheres in p and p part of w.</obo:IAO_0000115>
        <obo:IAO_0000119 rdf:resource="http://www.ncbi.nlm.nih.gov/pubmed/20064205"/>
        <obo:IAO_0000412 rdf:resource="http://purl.obolibrary.org/obo/ro.owl"/>
        <rdfs:label xml:lang="en">inheres in part of</rdfs:label>
    </owl:ObjectProperty>
    


    <!-- http://purl.obolibrary.org/obo/RO_0002320 -->

    <owl:ObjectProperty rdf:about="http://purl.obolibrary.org/obo/RO_0002320">
        <obo:IAO_0000115>A relationship that holds via some environmental process</obo:IAO_0000115>
        <obo:IAO_0000412 rdf:resource="http://purl.obolibrary.org/obo/ro.owl"/>
        <rdfs:label xml:lang="en">evolutionarily related to</rdfs:label>
    </owl:ObjectProperty>
    


    <!-- http://purl.obolibrary.org/obo/RO_0002323 -->

    <owl:ObjectProperty rdf:about="http://purl.obolibrary.org/obo/RO_0002323">
        <obo:IAO_0000115>A mereological relationship or a topological relationship</obo:IAO_0000115>
        <obo:IAO_0000412 rdf:resource="http://purl.obolibrary.org/obo/ro.owl"/>
        <rdfs:label xml:lang="en">mereotopologically related to</rdfs:label>
    </owl:ObjectProperty>
    


    <!-- http://purl.obolibrary.org/obo/RO_0002328 -->

    <owl:ObjectProperty rdf:about="http://purl.obolibrary.org/obo/RO_0002328">
        <obo:IAO_0000115>A grouping relationship for any relationship directly involving a function, or that holds because of a function of one of the related entities.</obo:IAO_0000115>
        <obo:IAO_0000412 rdf:resource="http://purl.obolibrary.org/obo/ro.owl"/>
        <rdfs:label xml:lang="en">functionally related to</rdfs:label>
    </owl:ObjectProperty>
    


    <!-- http://purl.obolibrary.org/obo/RO_0002350 -->

    <owl:ObjectProperty rdf:about="http://purl.obolibrary.org/obo/RO_0002350">
        <rdfs:subPropertyOf rdf:resource="http://purl.obolibrary.org/obo/BFO_0000050"/>
        <obo:IAO_0000115>is member of is a mereological relation between a item and a collection.</obo:IAO_0000115>
        <obo:IAO_0000119>SIO</obo:IAO_0000119>
        <obo:IAO_0000412 rdf:resource="http://purl.obolibrary.org/obo/ro.owl"/>
        <rdfs:label xml:lang="en">member of</rdfs:label>
    </owl:ObjectProperty>
    


    <!-- http://purl.obolibrary.org/obo/RO_0002351 -->

    <owl:ObjectProperty rdf:about="http://purl.obolibrary.org/obo/RO_0002351">
        <rdfs:subPropertyOf rdf:resource="http://purl.obolibrary.org/obo/BFO_0000051"/>
        <rdf:type rdf:resource="http://www.w3.org/2002/07/owl#IrreflexiveProperty"/>
        <obo:IAO_0000115>has member is a mereological relation between a collection and an item.</obo:IAO_0000115>
        <obo:IAO_0000119>SIO</obo:IAO_0000119>
        <obo:IAO_0000412 rdf:resource="http://purl.obolibrary.org/obo/ro.owl"/>
        <rdfs:label xml:lang="en">has member</rdfs:label>
    </owl:ObjectProperty>
    


    <!-- http://purl.obolibrary.org/obo/RO_0002352 -->

    <owl:ObjectProperty rdf:about="http://purl.obolibrary.org/obo/RO_0002352">
        <rdfs:subPropertyOf rdf:resource="http://purl.obolibrary.org/obo/RO_0000056"/>
        <rdfs:subPropertyOf rdf:resource="http://purl.obolibrary.org/obo/RO_0002328"/>
        <obo:IAO_0000115>inverse of has input</obo:IAO_0000115>
        <obo:IAO_0000412 rdf:resource="http://purl.obolibrary.org/obo/ro.owl"/>
        <rdfs:label xml:lang="en">input of</rdfs:label>
    </owl:ObjectProperty>
    


    <!-- http://purl.obolibrary.org/obo/RO_0002353 -->

    <owl:ObjectProperty rdf:about="http://purl.obolibrary.org/obo/RO_0002353">
        <rdfs:subPropertyOf rdf:resource="http://purl.obolibrary.org/obo/RO_0000056"/>
        <rdfs:subPropertyOf rdf:resource="http://purl.obolibrary.org/obo/RO_0002328"/>
        <obo:IAO_0000115>inverse of has output</obo:IAO_0000115>
        <obo:IAO_0000412 rdf:resource="http://purl.obolibrary.org/obo/ro.owl"/>
        <rdfs:label xml:lang="en">output of</rdfs:label>
    </owl:ObjectProperty>
    


    <!-- http://purl.obolibrary.org/obo/RO_0002354 -->

    <owl:ObjectProperty rdf:about="http://purl.obolibrary.org/obo/RO_0002354">
        <rdfs:subPropertyOf rdf:resource="http://purl.obolibrary.org/obo/RO_0002353"/>
        <obo:IAO_0000412 rdf:resource="http://purl.obolibrary.org/obo/ro.owl"/>
        <rdfs:label xml:lang="en">formed as result of</rdfs:label>
    </owl:ObjectProperty>
    


    <!-- http://purl.obolibrary.org/obo/RO_0002410 -->

    <owl:ObjectProperty rdf:about="http://purl.obolibrary.org/obo/RO_0002410">
        <obo:IAO_0000114 rdf:resource="http://purl.obolibrary.org/obo/IAO_0000428"/>
        <obo:IAO_0000115>This relation groups causal relations between material entities and causal relations between processes</obo:IAO_0000115>
        <obo:IAO_0000412 rdf:resource="http://purl.obolibrary.org/obo/ro.owl"/>
        <rdfs:label xml:lang="en">causally related to</rdfs:label>
    </owl:ObjectProperty>
    


    <!-- http://purl.obolibrary.org/obo/RO_0002473 -->

    <owl:ObjectProperty rdf:about="http://purl.obolibrary.org/obo/RO_0002473">
        <rdfs:subPropertyOf rdf:resource="http://purl.obolibrary.org/obo/BFO_0000051"/>
        <obo:IAO_0000115>x composed_primarily_of y if and only if more than half of the mass of x is made from y or units of the same type as y.</obo:IAO_0000115>
        <obo:IAO_0000119 rdf:resource="http://www.ncbi.nlm.nih.gov/pubmed/22293552"/>
        <obo:IAO_0000412 rdf:resource="http://purl.obolibrary.org/obo/ro.owl"/>
        <rdfs:label>composed primarily of</rdfs:label>
    </owl:ObjectProperty>
    


    <!-- http://purl.obolibrary.org/obo/RO_0002500 -->

    <owl:ObjectProperty rdf:about="http://purl.obolibrary.org/obo/RO_0002500">
        <rdfs:subPropertyOf rdf:resource="http://purl.obolibrary.org/obo/RO_0002595"/>
        <obo:IAO_0000115>A relationship between a material entity and a process where the material entity has some causal role that influences the process</obo:IAO_0000115>
        <obo:IAO_0000119 rdf:resource="http://purl.obolibrary.org/obo/ro/docs/causal-relations"/>
        <obo:IAO_0000412 rdf:resource="http://purl.obolibrary.org/obo/ro.owl"/>
        <rdfs:label>causal agent in process</rdfs:label>
    </owl:ObjectProperty>
    


    <!-- http://purl.obolibrary.org/obo/RO_0002502 -->

    <owl:ObjectProperty rdf:about="http://purl.obolibrary.org/obo/RO_0002502">
        <obo:IAO_0000412 rdf:resource="http://purl.obolibrary.org/obo/ro.owl"/>
        <rdfs:label>depends on</rdfs:label>
    </owl:ObjectProperty>
    


    <!-- http://purl.obolibrary.org/obo/RO_0002595 -->

    <owl:ObjectProperty rdf:about="http://purl.obolibrary.org/obo/RO_0002595">
        <rdfs:subPropertyOf rdf:resource="http://purl.obolibrary.org/obo/RO_0002410"/>
        <obo:IAO_0000115>A relationship that holds between a material entity and a process in which causality is involved, with either the material entity or some part of the material entity exerting some influence over the process, or the process influencing some aspect of the material entity.</obo:IAO_0000115>
        <obo:IAO_0000119 rdf:resource="http://purl.obolibrary.org/obo/ro/docs/causal-relations"/>
        <obo:IAO_0000412 rdf:resource="http://purl.obolibrary.org/obo/ro.owl"/>
        <rdfs:label>causal relation between material entity and a process</rdfs:label>
    </owl:ObjectProperty>
    


    <!-- http://purl.obolibrary.org/obo/RO_0002608 -->

    <owl:ObjectProperty rdf:about="http://purl.obolibrary.org/obo/RO_0002608">
        <rdfs:subPropertyOf rdf:resource="http://purl.obolibrary.org/obo/RO_0002410"/>
        <obo:IAO_0000115>Inverse of &apos;causal agent in process&apos;</obo:IAO_0000115>
        <obo:IAO_0000119 rdf:resource="http://purl.obolibrary.org/obo/ro/docs/causal-relations"/>
        <obo:IAO_0000412 rdf:resource="http://purl.obolibrary.org/obo/ro.owl"/>
        <rdfs:label>process has causal agent</rdfs:label>
    </owl:ObjectProperty>
    


    <!-- http://purl.obolibrary.org/obo/RO_0003001 -->

    <owl:ObjectProperty rdf:about="http://purl.obolibrary.org/obo/RO_0003001">
        <obo:IAO_0000114 rdf:resource="http://purl.obolibrary.org/obo/IAO_0000125"/>
        <obo:IAO_0000115>a produced_by b iff some process that occurs_in b has_output a.</obo:IAO_0000115>
        <obo:IAO_0000412 rdf:resource="http://purl.obolibrary.org/obo/ro.owl"/>
        <rdfs:label xml:lang="en">produced by</rdfs:label>
    </owl:ObjectProperty>
    


    <!-- http://purl.obolibrary.org/obo/RO_0003302 -->

    <owl:ObjectProperty rdf:about="http://purl.obolibrary.org/obo/RO_0003302">
        <rdfs:subPropertyOf rdf:resource="http://purl.obolibrary.org/obo/RO_0002410"/>
        <obo:IAO_0000115>A relationship between an entity (e.g. a genotype, genetic variation, chemical, or environmental exposure) and a condition (a phenotype or disease), where the entity has some causal or contributing role that influences the condition.</obo:IAO_0000115>
        <obo:IAO_0000412 rdf:resource="http://purl.obolibrary.org/obo/ro.owl"/>
        <rdfs:label xml:lang="en">causes or contributes to condition</rdfs:label>
    </owl:ObjectProperty>
    


    <!-- http://purl.obolibrary.org/obo/RO_0009001 -->

    <owl:ObjectProperty rdf:about="http://purl.obolibrary.org/obo/RO_0009001">
        <rdf:type rdf:resource="http://www.w3.org/2002/07/owl#IrreflexiveProperty"/>
        <obo:IAO_0000114 rdf:resource="http://purl.obolibrary.org/obo/IAO_0000428"/>
        <obo:IAO_0000115 xml:lang="en">&quot;has substance added&quot; is a relation existing between a (physical) entity and a substance in which the entity has had the substance added to it at some point in time.</obo:IAO_0000115>
        <obo:IAO_0000412 rdf:resource="http://purl.obolibrary.org/obo/ro.owl"/>
        <rdfs:label xml:lang="en">has substance added</rdfs:label>
    </owl:ObjectProperty>
    


    <!-- http://purl.obolibrary.org/obo/RO_0009002 -->

    <owl:ObjectProperty rdf:about="http://purl.obolibrary.org/obo/RO_0009002">
        <rdf:type rdf:resource="http://www.w3.org/2002/07/owl#IrreflexiveProperty"/>
        <obo:IAO_0000114 rdf:resource="http://purl.obolibrary.org/obo/IAO_0000428"/>
        <obo:IAO_0000115 xml:lang="en">&quot;has substance removed&quot; is a relation existing between two physical entities in which the first entity has had the second entity (a substance) removed from it at some point in time.</obo:IAO_0000115>
        <obo:IAO_0000412 rdf:resource="http://purl.obolibrary.org/obo/ro.owl"/>
        <rdfs:label xml:lang="en">has substance removed</rdfs:label>
    </owl:ObjectProperty>
    


    <!-- http://purl.obolibrary.org/obo/RO_0009003 -->

    <owl:ObjectProperty rdf:about="http://purl.obolibrary.org/obo/RO_0009003">
        <rdf:type rdf:resource="http://www.w3.org/2002/07/owl#IrreflexiveProperty"/>
        <obo:IAO_0000114 rdf:resource="http://purl.obolibrary.org/obo/IAO_0000428"/>
        <obo:IAO_0000115 xml:lang="en">&quot;immersed in&quot; is a relation between a (physical) entity and a fluid substance in which the entity is wholely or substantially surrounded by the substance.</obo:IAO_0000115>
        <obo:IAO_0000412 rdf:resource="http://purl.obolibrary.org/obo/ro.owl"/>
        <rdfs:label xml:lang="en">immersed in</rdfs:label>
    </owl:ObjectProperty>
    


    <!-- http://purl.obolibrary.org/obo/RO_0009004 -->

    <owl:ObjectProperty rdf:about="http://purl.obolibrary.org/obo/RO_0009004">
        <obo:IAO_0000114 rdf:resource="http://purl.obolibrary.org/obo/IAO_0000428"/>
        <obo:IAO_0000115 xml:lang="en">&apos;has consumer&apos; is a relation between a material entity and an organism in which the former can normally be digested or otherwise absorbed by the latter without immediate or persistent ill effect.</obo:IAO_0000115>
        <obo:IAO_0000412 rdf:resource="http://purl.obolibrary.org/obo/ro.owl"/>
        <rdfs:label xml:lang="en">has consumer</rdfs:label>
    </owl:ObjectProperty>
    


    <!-- http://purl.obolibrary.org/obo/RO_0009005 -->

    <owl:ObjectProperty rdf:about="http://purl.obolibrary.org/obo/RO_0009005">
        <rdfs:subPropertyOf rdf:resource="http://purl.obolibrary.org/obo/RO_0009001"/>
        <rdf:type rdf:resource="http://www.w3.org/2002/07/owl#IrreflexiveProperty"/>
        <obo:IAO_0000114 rdf:resource="http://purl.obolibrary.org/obo/IAO_0000428"/>
        <obo:IAO_0000115 xml:lang="en">&apos;has primary substance added&apos; indicates that an entity has had the given substance added to it in a proportion greater than any other added substance.</obo:IAO_0000115>
        <obo:IAO_0000412 rdf:resource="http://purl.obolibrary.org/obo/ro.owl"/>
        <rdfs:label xml:lang="en">has primary substance added</rdfs:label>
    </owl:ObjectProperty>
    


    <!-- http://purl.obolibrary.org/obo/RO_HOM0000000 -->

    <owl:ObjectProperty rdf:about="http://purl.obolibrary.org/obo/RO_HOM0000000">
        <rdf:type rdf:resource="http://www.w3.org/2002/07/owl#SymmetricProperty"/>
        <obo:IAO_0000115 rdf:datatype="http://www.w3.org/2001/XMLSchema#string">Relation between biological objects that resemble or are related to each other sufficiently to warrant a comparison.</obo:IAO_0000115>
        <obo:IAO_0000412 rdf:resource="http://purl.obolibrary.org/obo/ro.owl"/>
        <rdfs:label rdf:datatype="http://www.w3.org/2001/XMLSchema#string">in similarity relationship with</rdfs:label>
    </owl:ObjectProperty>
    


    <!-- http://www.w3.org/2002/07/owl#topObjectProperty -->

    <owl:ObjectProperty rdf:about="http://www.w3.org/2002/07/owl#topObjectProperty">
        <obo:IAO_0000412 rdf:resource="http://purl.obolibrary.org/obo/ro.owl"/>
    </owl:ObjectProperty>
    


    <!-- 
    ///////////////////////////////////////////////////////////////////////////////////////
    //
    // Classes
    //
    ///////////////////////////////////////////////////////////////////////////////////////
     -->

    


    <!-- http://purl.obolibrary.org/obo/BFO_0000002 -->

    <owl:Class rdf:about="http://purl.obolibrary.org/obo/BFO_0000002">
        <obo:IAO_0000115 xml:lang="en">An entity that exists in full at any time in which it exists at all, persists through time while maintaining its identity and has no temporal parts.</obo:IAO_0000115>
        <obo:IAO_0000412 rdf:resource="http://purl.obolibrary.org/obo/ro.owl"/>
        <rdfs:label xml:lang="en">continuant</rdfs:label>
    </owl:Class>
    


    <!-- http://purl.obolibrary.org/obo/BFO_0000004 -->

    <owl:Class rdf:about="http://purl.obolibrary.org/obo/BFO_0000004">
        <rdfs:subClassOf rdf:resource="http://purl.obolibrary.org/obo/BFO_0000002"/>
        <obo:IAO_0000115 xml:lang="en">A continuant that is a bearer of quality and realizable entity entities, in which other entities inhere and which itself cannot inhere in anything.</obo:IAO_0000115>
        <obo:IAO_0000412 rdf:resource="http://purl.obolibrary.org/obo/ro.owl"/>
        <rdfs:label xml:lang="en">independent continuant</rdfs:label>
    </owl:Class>
    


    <!-- http://purl.obolibrary.org/obo/BFO_0000040 -->

    <owl:Class rdf:about="http://purl.obolibrary.org/obo/BFO_0000040">
        <rdfs:subClassOf rdf:resource="http://purl.obolibrary.org/obo/BFO_0000004"/>
        <obo:IAO_0000115 xml:lang="en">An independent continuant that is spatially extended whose identity is independent of that of other entities and can be maintained through time.</obo:IAO_0000115>
        <obo:IAO_0000412 rdf:resource="http://purl.obolibrary.org/obo/ro.owl"/>
        <rdfs:label xml:lang="en">material entity</rdfs:label>
    </owl:Class>
    


    <!-- http://purl.obolibrary.org/obo/RO_0002577 -->

    <owl:Class rdf:about="http://purl.obolibrary.org/obo/RO_0002577">
        <rdfs:subClassOf rdf:resource="http://purl.obolibrary.org/obo/BFO_0000040"/>
        <obo:IAO_0000115>A material entity consisting of multiple components that are causally integrated.</obo:IAO_0000115>
        <obo:IAO_0000119>http://www.jbiomedsem.com/content/4/1/43</obo:IAO_0000119>
        <obo:IAO_0000412 rdf:resource="http://purl.obolibrary.org/obo/ro.owl"/>
        <rdfs:label>system</rdfs:label>
    </owl:Class>
</rdf:RDF>



<!-- Generated by the OWL API (version 4.5.6) https://github.com/owlcs/owlapi -->

